              x(=s)
            a(=t)   b
          a1 a2     


(1)
          a(=t')
        a1     small

(2)
          x(=s')
       big      b

(small, big) = partition pivot a2

--

A(s)
= T(s) + P(t') + P(s') - P(s)
= 1 + T(a2) + P(t') + P(s') - P(s)
= 1 + A(a2) - P(small) - P(big) + P(a2) + P(t') + P(s') - P(s)
  (
    P(t') = p(t') + P(a1) + P(small)
    P(s') = p(s') + P(big) + P(b)
    P(s) = p(s) + P(t) + P(b)
  )
= 1 + A(a2) - P(small) - P(big) + P(a2) + p(t') + P(a1) + P(small) + p(s') + P(big) + P(b) - (p(s) + P(t) + P(b))
= 1 + A(a2) + P(a2) + p(t') + P(a1) + p(s') - (p(s) + P(t))
= 1 + A(a2) + P(a2) + P(a1) + p(t') + p(s') - p(s) - P(t)
  (
    P(t) = p(t) + P(a1) + P(a2)
    => P(a1) + P(a2) = P(t) - p(t)
  )
= 1 + A(a2) + P(t) - p(t) + p(t') + p(s') - p(s) - P(t)
= 1 + A(a2) - p(t) + p(t') + p(s') - p(s)
<= 2 + 2*p(a2) + p(t') + p(s') - p(s) - p(t)
  (
    p(s') <= p(s)
    p(a2) < p(t)
  )
< 2 + 2*p(a2) + p(t') + p(s') - p(s) - p(t)
= 1 + 1 + p(a2) + p(t')
< 1 + 2p(s)
